\paragraph{Addition}

Addition of two points \(P + Q = R\) is a fairly straight-forward matter. Given two points, \(P = (x_1,y_1)\) and
\(Q = (x_2,y_2)\), the result \(R = (x_3,y_3)\) can be found with the following calculations:

\begin{equation}
	\lambda = {{y_2-y_1} \over {x_2-x_1}}
\end{equation}

\begin{equation}
	x_3 = \lambda^2 - x_1 - x_2 \textbf{ and } y_3 = \lambda (x_1 - x_3) - y_1
\end{equation}

As elliptic curves also contain the \(\infty\) (infinity) point, there is a single exception to this
rule: \(Q = \infty \lor P = \infty \implies P + Q = \infty\) (if either \(P\) or \(Q\) is infinity,
the result of adding them will be infinity, too).

\paragraph{Subtraction}

A subtraction \(P - Q = R\) can be expressed through addition and negation, as \(P - Q = P + (-Q)\). Negation of a given
\(P = (x,y)\) is calculated as \(-P = (x,-y)\). Subtraction can then be calculated as \((x_1,y_1) - (x_2,y_2) = (x_3,-y_3)\).

As with addition, negation is complicated by the existence of the infinity point. The negation of infinity is infinity (negative
infinity does not exist), and a point subtracted from itself is infinity:

\begin{equation}
	-\infty = \infty \textbf{ and } P - P = \infty
\end{equation}

\paragraph{Doubling}

Used if \(Q = P\) in \(P + Q\). Guide... p. 80 (quote)
\begin{quote}
	Let P = (x1,y1) in E(K), where P not= -P. Then 2P = (x3,y3), where
	
	x3 = ((3x1\^2+a)/(2y1))\^2-2x1    and    y3 = ((3x1\^2+a)/2y1)*(x1-x3)-y1
\end{quote}

Note: All of this is from Hakerson p. 80.